Tweak FStar.Bytes.fsti

ulib/FStar.Bytes.fsti
@@ -127,11 +127,12 @@ val init:
   -> f:(i:u32{U32.(i <^ len)} -> byte)
   -> b:lbytes (U32.v len){forall (i:u32{U32.(i <^ len)}).{:pattern b.[i]} b.[i] = f i}
 
-let abyte (b:byte) : lbytes 1 =
-    admit () (* create 1ul b *)
+// this is a hack JROESCH
+val abyte (b:byte) : lbytes 1
+    (* admit () create 1ul b *)
 
-let twobytes (b:byte*byte) : lbytes 2 =
-    init 2ul (fun i -> if i = 0ul then fst b else snd b)
+val twobytes (b:byte*byte) : lbytes 2
+    (* init 2ul (fun i -> if i = 0ul then fst b else snd b) *)
 
 (** appending bytes **)
 val append:
